New typing rule And-I inspired by WFDOT, needed for Pathless Scala
The new rule is:

Γ ⊢ x: T     Γ ⊢ x: U
----------------------(And-I)
    Γ ⊢ x: T ∧ U

This rule existed in WadlerFest DOT but not in OOPSLA16 DOT. Adding it seems to
be necessary but not sufficient for preserving typing of selections on
intersection types in Pathless Scala [1].

Only the alternative soundness proof dot_soundness_alt.v was updated,
so dot_soundness.v doesn't typecheck anymore.

[1]: http://guillaume.martres.me/pathless-scala.pdf

oopsla16/dot.v
@@ -258,6 +258,10 @@ Inductive has_type : tenv -> venv -> tm -> ty -> nat -> Prop :=
       has_type GH G1 t T1 n1 ->
       stp GH G1 T1 T2 n2 ->
       has_type GH G1 t T2 (S (n1 + n2))
+  | T_AndI : forall GH G1 b x T1 T2 n1 n2,
+      has_type GH G1 (tvar b x) T1 n1 ->
+      has_type GH G1 (tvar b x) T2 n2 ->
+      has_type GH G1 (tvar b x) (TAnd T1 T2) (S (n1+n2))
 
 (* : -- member initialization *)
 with dms_has_type: tenv -> venv -> dms -> ty -> nat -> Prop :=
@@ -606,6 +610,7 @@ Proof.
   - econstructor. subst. eapply IHn. eauto. omega. eapply IHn. eauto. omega. eapply closed_extend. eauto.
   - eapply T_AppVar. eapply IHn. eauto. omega. eapply IHn. eauto. omega. eauto. eapply closed_extend. eauto.
   - econstructor. eapply IHn. eauto. omega. eapply IHn. eauto. omega.
+  - eapply T_AndI. eapply IHn. eauto. omega. eapply IHn. eauto. omega.
   (* dms_has_type *)
   - econstructor.
   - econstructor. eapply IHn. eauto. omega. eapply closed_extend. eauto. eauto. eauto.
@@ -742,6 +747,7 @@ Proof.
   - eapply IHT in H1. inversion H1. eauto. omega.
   - eapply IHT in H1. inversion H1. eauto. omega.
   - eapply IHS2. eauto. omega.
+  - econstructor. eapply IHT. eapply H1. omega. eapply IHT. eapply H2. omega.
   (* dms_has_type *)
   - econstructor.
   - subst. econstructor. econstructor. eauto. eauto. eapply IHD. eauto. omega.
